src/InlineFacts_2.v
@@ -359,7 +359,7 @@ Proof.
   simpl in Heqoattr.
   apply getAttribute_Some_body in Heqoattr.
   simpl; inv H.
-  pose proof (MethsEquiv_in _ H1 Heqoattr).
+  pose proof (proj1 (MethsEquiv_in type typeUT (getDefsBodies m)) H1 _ Heqoattr).
   constructor.
   - apply inlineDmToRules_RulesEquiv; auto.
   - apply inlineDmToDms_MethsEquiv; auto.
