src/ParametricEquiv.v
@@ -1,0 +1,157 @@
+Require Import ParametricSyntax Syntax List Lib.CommonTactics.
+
+Section Equiv.
+  Variable t1 t2: Kind -> Type.
+
+  Definition ft1 := fullType t1.
+  Definition ft2 := fullType t2.
+  Hint Unfold ft1 ft2.
+
+  Inductive GenActionEquiv: forall {k}, GenActionT t1 k -> GenActionT t2 k -> Prop :=
+  | GAEMCall: forall {k} n s (e1: Expr t1 (SyntaxKind (arg s)))
+                     (e2: Expr t2 (SyntaxKind (arg s)))
+                     (cont1: t1 (ret s) -> GenActionT t1 k)
+                     (cont2: t2 (ret s) -> GenActionT t2 k),
+                (forall (v1: ft1 (SyntaxKind (ret s)))
+                        (v2: ft2 (SyntaxKind (ret s))),
+                   GenActionEquiv (cont1 v1) (cont2 v2)) ->
+                GenActionEquiv (GMCall n s e1 cont1) (GMCall n s e2 cont2)
+  | GAELet: forall {k k1' k2'} (e1: Expr t1 k1') (e2: Expr t2 k2')
+                   (cont1: fullType t1 k1' -> GenActionT t1 k)
+                   (cont2: fullType t2 k2' -> GenActionT t2 k),
+              (forall (v1: ft1 k1') (v2: ft2 k2'),
+                 GenActionEquiv (cont1 v1) (cont2 v2)) ->
+              GenActionEquiv (GLet_ e1 cont1) (GLet_ e2 cont2)
+  | GAEReadReg: forall {k k1' k2'} rn
+                       (cont1: fullType t1 k1' -> GenActionT t1 k)
+                       (cont2: fullType t2 k2' -> GenActionT t2 k),
+                  (forall (v1: ft1 k1') (v2: ft2 k2'),
+                     GenActionEquiv (cont1 v1) (cont2 v2)) ->
+                  GenActionEquiv (GReadReg rn _ cont1) (GReadReg rn _ cont2)
+  | GAEWriteReg: forall {k k1' k2'} rn (e1: Expr t1 k1') (e2: Expr t2 k2')
+                        (cont1: GenActionT t1 k) (cont2: GenActionT t2 k),
+                   (* ExprEquiv G e1 e2 -> *)
+                   GenActionEquiv cont1 cont2 ->
+                   GenActionEquiv (GWriteReg rn e1 cont1) (GWriteReg rn e2 cont2)
+  | GAEIfElse: forall {k k'} (e1: Expr t1 (SyntaxKind Bool)) (e2: Expr t2 (SyntaxKind Bool))
+                      (ta1 fa1: GenActionT t1 k') (ta2 fa2: GenActionT t2 k')
+                      (cont1: t1 k' -> GenActionT t1 k) (cont2: t2 k' -> GenActionT t2 k),
+                 (* ExprEquiv G e1 e2 -> *)
+                 GenActionEquiv ta1 ta2 -> GenActionEquiv fa1 fa2 ->
+                 (forall (v1: ft1 (SyntaxKind k')) (v2: ft2 (SyntaxKind k')),
+                    GenActionEquiv (cont1 v1) (cont2 v2)) ->
+                 GenActionEquiv (GIfElse e1 ta1 fa1 cont1) (GIfElse e2 ta2 fa2 cont2)
+  | GAEAssert: forall {k} (e1: Expr t1 (SyntaxKind Bool)) (e2: Expr t2 (SyntaxKind Bool))
+                      (cont1: GenActionT t1 k) (cont2: GenActionT t2 k),
+                 (* ExprEquiv G e1 e2 -> *)
+                 GenActionEquiv cont1 cont2 ->
+                 GenActionEquiv (GAssert_ e1 cont1) (GAssert_ e2 cont2)
+  | GAERet: forall {k} (e1: Expr t1 (SyntaxKind k))
+                   (e2: Expr t2 (SyntaxKind k)),
+              (* ExprEquiv G e1 e2 -> *)
+              GenActionEquiv (GReturn e1) (GReturn e2).
+  
+  Inductive SinActionEquiv: forall {k}, SinActionT t1 k -> SinActionT t2 k -> Prop :=
+  | SAEMCall: forall {k} n s (e1: Expr t1 (SyntaxKind (arg s)))
+                     (e2: Expr t2 (SyntaxKind (arg s)))
+                     (cont1: t1 (ret s) -> SinActionT t1 k)
+                     (cont2: t2 (ret s) -> SinActionT t2 k),
+                (forall (v1: ft1 (SyntaxKind (ret s)))
+                        (v2: ft2 (SyntaxKind (ret s))),
+                   SinActionEquiv (cont1 v1) (cont2 v2)) ->
+                SinActionEquiv (SMCall n s e1 cont1) (SMCall n s e2 cont2)
+  | SAELet: forall {k k1' k2'} (e1: Expr t1 k1') (e2: Expr t2 k2')
+                   (cont1: fullType t1 k1' -> SinActionT t1 k)
+                   (cont2: fullType t2 k2' -> SinActionT t2 k),
+              (forall (v1: ft1 k1') (v2: ft2 k2'),
+                 SinActionEquiv (cont1 v1) (cont2 v2)) ->
+              SinActionEquiv (SLet_ e1 cont1) (SLet_ e2 cont2)
+  | SAEReadReg: forall {k k1' k2'} rn
+                       (cont1: fullType t1 k1' -> SinActionT t1 k)
+                       (cont2: fullType t2 k2' -> SinActionT t2 k),
+                  (forall (v1: ft1 k1') (v2: ft2 k2'),
+                     SinActionEquiv (cont1 v1) (cont2 v2)) ->
+                  SinActionEquiv (SReadReg rn _ cont1) (SReadReg rn _ cont2)
+  | SAEWriteReg: forall {k k1' k2'} rn (e1: Expr t1 k1') (e2: Expr t2 k2')
+                        (cont1: SinActionT t1 k) (cont2: SinActionT t2 k),
+                   (* ExprEquiv G e1 e2 -> *)
+                   SinActionEquiv cont1 cont2 ->
+                   SinActionEquiv (SWriteReg rn e1 cont1) (SWriteReg rn e2 cont2)
+  | SAEIfElse: forall {k k'} (e1: Expr t1 (SyntaxKind Bool)) (e2: Expr t2 (SyntaxKind Bool))
+                      (ta1 fa1: SinActionT t1 k') (ta2 fa2: SinActionT t2 k')
+                      (cont1: t1 k' -> SinActionT t1 k) (cont2: t2 k' -> SinActionT t2 k),
+                 (* ExprEquiv G e1 e2 -> *)
+                 SinActionEquiv ta1 ta2 -> SinActionEquiv fa1 fa2 ->
+                 (forall (v1: ft1 (SyntaxKind k')) (v2: ft2 (SyntaxKind k')),
+                    SinActionEquiv (cont1 v1) (cont2 v2)) ->
+                 SinActionEquiv (SIfElse e1 ta1 fa1 cont1) (SIfElse e2 ta2 fa2 cont2)
+  | SAEAssert: forall {k} (e1: Expr t1 (SyntaxKind Bool)) (e2: Expr t2 (SyntaxKind Bool))
+                      (cont1: SinActionT t1 k) (cont2: SinActionT t2 k),
+                 (* ExprEquiv G e1 e2 -> *)
+                 SinActionEquiv cont1 cont2 ->
+                 SinActionEquiv (SAssert_ e1 cont1) (SAssert_ e2 cont2)
+  | SAERet: forall {k} (e1: Expr t1 (SyntaxKind k))
+                   (e2: Expr t2 (SyntaxKind k)),
+              (* ExprEquiv G e1 e2 -> *)
+              SinActionEquiv (SReturn e1) (SReturn e2).
+
+  Definition MetaRuleEquiv r :=
+    match r with
+      | OneRule b s => SinActionEquiv (b t1) (b t2)
+      | RepRule _ _ _ _ bgen s _ => GenActionEquiv (bgen t1) (bgen t2)
+    end.
+
+  Inductive MetaRulesEquiv: list MetaRule -> Prop :=
+  | MetaRulesEquivNil: MetaRulesEquiv nil
+  | MetaRulesEquivCons:
+      forall r,
+        MetaRuleEquiv r ->
+        forall rules,
+          MetaRulesEquiv rules -> MetaRulesEquiv (r :: rules).
+
+  Lemma MetaRulesEquiv_in:
+    forall rules,
+      MetaRulesEquiv rules <-> (forall r, In r rules -> MetaRuleEquiv r).
+  Proof.
+    intros; constructor.
+    - induction 1; intros; intuition.
+      inv H1; auto.
+    - induction rules; intros; simpl in *; auto.
+      + constructor.
+      + assert (sth: forall r, In r rules -> MetaRuleEquiv r) by intuition.
+        specialize (IHrules sth).
+        assert (sth2: MetaRuleEquiv a) by intuition.
+        constructor; auto.
+  Qed.
+  
+  Definition MetaMethEquiv r :=
+    match r with
+      | OneMeth b s => forall v1 v2, SinActionEquiv (projT2 b t1 v1) (projT2 b t2 v2)
+      | RepMeth _ _ _ _ bgen s _ => forall v1 v2, GenActionEquiv (projT2 bgen t1 v1)
+                                                                 (projT2 bgen t2 v2)
+    end.
+
+  Inductive MetaMethsEquiv: list MetaMeth -> Prop :=
+  | MetaMethsEquivNil: MetaMethsEquiv nil
+  | MetaMethsEquivCons:
+      forall dm, MetaMethEquiv dm ->
+                 forall meths,
+                   MetaMethsEquiv meths -> MetaMethsEquiv (dm :: meths).
+
+  Lemma MetaMethsEquiv_in:
+    forall meths,
+      MetaMethsEquiv meths <-> (forall m, In m meths -> MetaMethEquiv m).
+  Proof.
+    intros; constructor.
+    - induction 1; intros; intuition.
+      inv H1; auto.
+    - induction meths; intros; simpl in *; auto.
+      + constructor.
+      + assert (sth: forall m, In m meths -> MetaMethEquiv m) by intuition.
+        specialize (IHmeths sth).
+        assert (sth2: MetaMethEquiv a) by intuition.
+        constructor; auto.
+  Qed.
+  
+  Definition MetaModEquiv m := MetaRulesEquiv (metaRules m) /\ MetaMethsEquiv (metaMeths m).
+End Equiv.
