src/ParametricInline.v
@@ -1,0 +1,139 @@
+Require Import InlineFacts_2 ParametricSyntax ParametricEquiv Syntax String List Semantics.
+
+Section GenGen.
+  Variable m: MetaModule.
+  Variable mEquiv: forall ty, MetaModEquiv ty typeUT m.
+
+  Variable A: Type.
+  Variable strA: A -> string.
+  Variable goodStrFn: forall i j, strA i = strA j -> i = j.
+  Variable goodStrFn2: forall si sj i j, addIndexToStr strA i si = addIndexToStr strA j sj ->
+                                         si = sj /\ i = j.
+  Variable dm: sigT GenMethodT.
+  Variable dmName: string.
+  Variable ls: list A.
+
+  Variable r: GenAction Void.
+  Variable rName: string.
+
+  Hypotheses (Hdm: In (RepMeth strA goodStrFn goodStrFn2 dm dmName ls) (metaMeths m))
+             (HnoDupMeths: NoDup (map getMetaMethName (metaMeths m)))
+             (HnoDupRules: NoDup (map getMetaRuleName (metaRules m))).
+  Hypothesis Hrule: In (RepRule strA goodStrFn goodStrFn2 r rName ls) (metaRules m).
+
+  Lemma InlineGenGenDmToRule_traceRefines_1:
+    makeModule m <<==
+               makeModule
+               {| metaRegs := metaRegs m;
+                  metaRules :=
+                    map (fun newr =>
+                           if string_dec rName (getMetaRuleName newr)
+                           then RepRule strA goodStrFn goodStrFn2
+                                        (fun ty => inlineGenGenDm (r ty) dmName dm) rName ls
+                           else newr) (metaRules m);
+                  metaMeths := metaMeths m |}.
+  Proof.
+    admit.
+  Qed.
+
+  Hypothesis HnoRuleCalls: forall rule,
+                             In rule (metaRules m) ->
+                             getMetaRuleName rule <> rName ->
+                             ~ In dmName (map (fun n => nameVal (nameRec n))
+                                              (getCallsMetaRule rule)).
+
+  Hypothesis HnoMethCalls: forall meth,
+                             In meth (metaMeths m) ->
+                             getMetaMethName meth <> dmName ->
+                             ~ In dmName (map (fun n => nameVal (nameRec n))
+                                              (getCallsMetaMeth meth)).
+  
+  Lemma inlineGenGenDmToRule_traceRefines_2:
+    makeModule m <<==
+               makeModule
+               {| metaRegs := metaRegs m;
+                  metaRules :=
+                    map (fun newr =>
+                           if string_dec rName (getMetaRuleName newr)
+                           then RepRule strA goodStrFn goodStrFn2
+                                        (fun ty => inlineGenGenDm (r ty) dmName dm) rName ls
+                           else newr) (metaRules m);
+                  metaMeths :=
+                    filter
+                      (fun dm' =>
+                         if string_dec dmName (getMetaMethName dm')
+                         then false
+                         else true) (metaMeths m) |}.
+  Proof.
+    admit.
+  Qed.
+End GenGen.
+
+Section GenSin.
+  Variable m: MetaModule.
+  Variable mEquiv: forall ty, MetaModEquiv ty typeUT m.
+
+  Variable A: Type.
+  Variable strA: A -> string.
+  Variable goodStrFn: forall i j, strA i = strA j -> i = j.
+  Variable goodStrFn2: forall si sj i j, addIndexToStr strA i si = addIndexToStr strA j sj ->
+                                         si = sj /\ i = j.
+  Variable dm: sigT SinMethodT.
+  Variable dmName: string.
+  Variable ls: list A.
+
+  Variable r: GenAction Void.
+  Variable rName: string.
+
+  Hypotheses (Hdm: In (OneMeth dm dmName) (metaMeths m))
+             (HnoDupMeths: NoDup (map getMetaMethName (metaMeths m)))
+             (HnoDupRules: NoDup (map getMetaRuleName (metaRules m))).
+  Hypothesis Hrule: In (RepRule strA goodStrFn goodStrFn2 r rName ls) (metaRules m).
+
+  Lemma InlineGenSinDmToRule_traceRefines_1:
+    makeModule m <<==
+               makeModule
+               {| metaRegs := metaRegs m;
+                  metaRules :=
+                    map (fun newr =>
+                           if string_dec rName (getMetaRuleName newr)
+                           then RepRule strA goodStrFn goodStrFn2
+                                        (fun ty => inlineGenSinDm (r ty) dmName dm) rName ls
+                           else newr) (metaRules m);
+                  metaMeths := metaMeths m |}.
+  Proof.
+    admit.
+  Qed.
+
+  Hypothesis HnoRuleCalls: forall rule,
+                             In rule (metaRules m) ->
+                             getMetaRuleName rule <> rName ->
+                             ~ In dmName (map (fun n => nameVal (nameRec n))
+                                              (getCallsMetaRule rule)).
+
+  Hypothesis HnoMethCalls: forall meth,
+                             In meth (metaMeths m) ->
+                             getMetaMethName meth <> dmName ->
+                             ~ In dmName (map (fun n => nameVal (nameRec n))
+                                              (getCallsMetaMeth meth)).
+  
+  Lemma inlineGenSinDmToRule_traceRefines_2:
+    makeModule m <<==
+               makeModule
+               {| metaRegs := metaRegs m;
+                  metaRules :=
+                    map (fun newr =>
+                           if string_dec rName (getMetaRuleName newr)
+                           then RepRule strA goodStrFn goodStrFn2
+                                        (fun ty => inlineGenSinDm (r ty) dmName dm) rName ls
+                           else newr) (metaRules m);
+                  metaMeths :=
+                    filter
+                      (fun dm' =>
+                         if string_dec dmName (getMetaMethName dm')
+                         then false
+                         else true) (metaMeths m) |}.
+  Proof.
+    admit.
+  Qed.
+End GenSin.
